proved equivalence of BFS version and facts about shortest paths

examples/graph/theories/BFSProofs.v
@@ -11,9 +11,17 @@ Require Import Coq.Lists.SetoidList.
 Require Import Omega.
 Require Import Wellfounded.
 Require Import Coq.Relations.Relation_Operators.
+Require Import Coq.Lists.ListDec.
 
 Require Import CoLoR.Util.Relation.Lexico.
 Require Import CoLoR.Util.Relation.SN.
+
+Require Import Coq.FSets.FMapList.
+Require Import Coq.FSets.FMapInterface.
+Require Import Coq.Structures.OrderedTypeEx.
+
+Module M := FMapList.Make(N_as_OT).
+
 
 (*Helpers*)
 Definition null {a} (l: list a) :=
@@ -22,6 +30,60 @@ Definition null {a} (l: list a) :=
   | _ => false
   end.
 
+Ltac simplify' := try(rewrite andb_diag in *); try(rewrite andb_true_iff in *); try(rewrite negb_true_iff in *);
+  try(rewrite andb_false_iff in *); try(rewrite negb_false_iff in *); intuition.
+
+Ltac destruct_all :=
+repeat(match goal with
+            |[H: (exists _, _) |- _] => destruct H
+            |[H: _ /\ _ |- _] => destruct H 
+            end; try(rewrite andb_true_iff in *)).
+
+(*Ltac for solving statements of the form: In x l, where l may be many lists appended together*) 
+Ltac solve_in :=
+  match goal with
+  | [ H : _ |- In ?x (?l ++ ?r)] => apply in_or_app; solve_in
+  | [ H : _ |- In ?x ?s \/ In ?x ?s'] => (right; solve_in) + (left; solve_in) 
+  | [ H : _ |- In ?x (?x :: ?l)] => simpl; left; reflexivity
+  | [H : _ |- In ?x (?a :: ?l)] => simpl; right; solve_in
+  | [ H : _ |- _ ] => try(reflexivity); assumption
+end. 
+
+Lemma in_split_app_fst: forall (A: Type) (l: list A) (x: A),
+  (forall x y : A, {x = y} + {x <> y}) ->
+  In x l ->
+  exists l1 l2, l = l1 ++ (x :: l2) /\ forall y, In y l1 -> y <> x.
+Proof.
+  intros. induction l.
+  - inversion H.
+  - destruct (X x a). subst. exists nil. exists l. split. reflexivity. intros. inversion H0.
+    simpl in H. destruct H. subst. contradiction.  apply IHl in H. destruct_all.
+    exists (a :: x0). exists x1. split. rewrite H. reflexivity. intros. intro. subst.
+    simpl in H1. destruct H1. subst. contradiction. apply H0 in H. contradiction.
+Qed.
+
+Lemma no_no_dup: forall (A: Type) (l: list A),
+  (forall x y : A, {x = y} + {x <> y}) ->
+  ~(NoDup l) <-> (exists w l1 l2 l3, l = l1 ++ w :: l2 ++ w :: l3).
+Proof.
+  intros. split; intros.
+  - induction l.
+    + assert (@NoDup A nil). constructor. contradiction.
+    + destruct (NoDup_dec X l).
+      * assert (In a l). destruct (In_dec X a l). apply i.
+        assert (NoDup (a :: l)). constructor. apply n0. apply n. contradiction.
+        apply in_split_app_fst in H0. destruct_all. exists a. exists nil. exists x. exists x0.
+        rewrite H0. reflexivity. apply X.
+      * apply IHl in n. destruct_all. exists x. exists (a :: x0). exists x1. exists x2. rewrite H0.
+        reflexivity.
+  -  intro. destruct_all.  subst. induction x0; simpl in *.
+    + rewrite NoDup_cons_iff in H0. destruct_all. apply H.
+    solve_in.
+    + simpl in H0. rewrite NoDup_cons_iff in H0. destruct_all. apply IHx0. apply H0.
+Qed.
+
+
+(*
 (*Function to pop off queue satisfying given predicate*)
 Fixpoint pop_list {a} (l: list a) (p: a -> bool) :=
   match l with
@@ -50,48 +112,129 @@ Proof.
   intros. induction l. simpl in H. inversion H. simpl in H. destruct (p a0) eqn : B.
   apply IHl. apply H. inversion H; subst; assumption.
 Qed.
-
+*)
 (* Inductive relation*)
 Section Ind.
 
 Context {a : Type} {b : Type} { gr : Type -> Type -> Type} {Hgraph : Graph.Graph gr} {Hlaw : Graph.LawfulGraph gr}.
 
-Definition state : Type := (gr a b) * list (Graph.Path) * RootPath.RTree.
+Section Lex.
+
+(*Well formed lexicographic measure - maybe put in own section*)
+Definition natNodes (g : gr a b) := (BinInt.Z.abs_nat(Graph.noNodes g)).
+
+Definition natNodes_lt x y := natNodes x < natNodes y.
+Definition natNodes_eq x y := natNodes x = natNodes y.
+Definition list_length_lt {a} (x y : list a) := length x < length y.
+Definition queue_length_lt  {a} (x y : Queue a) := list_length_lt (toList _ x) (toList _ y).
+
+Definition bf_measure_list (a: Type) := 
+  transp (lex (transp natNodes_lt) natNodes_eq (transp  (@list_length_lt a))).
+
+Definition bf_measure_queue (a: Type) :=
+  transp (lex (transp natNodes_lt) natNodes_eq (transp (@queue_length_lt a))).
+
+Definition f_nat_lt {a} (f: a -> nat) x y := f x < f y.
+
+Lemma f_nat_lt_acc: forall {a} (f: a -> nat) x n, f x <= n -> Acc (f_nat_lt f) x.
+Proof.
+  intros. generalize dependent x. induction n; auto.
+  - intros. apply Acc_intro. intros. unfold f_nat_lt in *. omega.
+  - unfold f_nat_lt in *. intros. apply Acc_intro. intros. apply IHn. omega.
+Qed.
+
+Lemma f_nat_lt_wf: forall {a} (f: a -> nat), well_founded (f_nat_lt f).
+Proof.
+  red. intro. intro. intro. eapply f_nat_lt_acc. eauto.
+Qed.
+
+
+Lemma wf_bf_measure_list : forall a,  WF (transp (bf_measure_list a)).
+Proof.
+  intros. eapply WF_lex.
+  - apply wf_transp_WF. unfold transp. 
+    pose proof (f_nat_lt_wf (natNodes)). unfold f_nat_lt in H. unfold natNodes_lt. apply H.
+  - apply wf_transp_WF. unfold transp.
+    pose proof (f_nat_lt_wf (@length a0)). unfold f_nat_lt in H. unfold natNodes_lt. apply H.
+  - unfold Transitive. intros. unfold natNodes_eq in *. omega.
+  - unfold inclusion. unfold RelUtil.compose. intros.
+    unfold transp in *. unfold natNodes_lt in *. unfold natNodes_eq in *. destruct H. omega.
+Qed.
+
+Lemma well_founded_bf_measure_list: forall a, well_founded (bf_measure_list a).
+Proof. 
+  intros.
+  apply WF_transp_wf. apply wf_bf_measure_list.
+Qed.
+
+Lemma wf_bf_measure_queue : forall a, WF (transp (bf_measure_queue a)).
+Proof.
+  intros.
+  eapply WF_lex.
+  - apply wf_transp_WF. unfold transp. 
+    pose proof (f_nat_lt_wf (natNodes)). unfold f_nat_lt in H. unfold natNodes_lt. apply H.
+  - apply wf_transp_WF. unfold transp.
+    pose proof (f_nat_lt_wf (fun x => length (toList a0 x))). unfold f_nat_lt in H. unfold queue_length_lt.
+    unfold list_length_lt. apply H.
+  - unfold Transitive. intros. unfold natNodes_eq in *. omega.
+  - unfold inclusion. unfold RelUtil.compose. intros.
+    unfold transp in *. unfold natNodes_lt in *. unfold natNodes_eq in *. destruct H. omega.
+Qed.
+
+Lemma well_founded_bf_measure_queue: forall a, well_founded (bf_measure_queue a).
+Proof.
+  intros.
+  apply WF_transp_wf. apply wf_bf_measure_queue.
+Qed.
+
+
+
+
+End Lex.
+
+Definition state : Type := (gr a b) * (list (Node * Num.Int)) * (list (Node * Num.Int)) * nat * (M.t nat).
   
 
 Definition get_graph (s: state) :=
   match s with
-  | (g, _, _) => g
+  | (g, _, _, _, _) => g
   end.
 
 Definition get_queue (s: state) :=
   match s with
-  | (_, q, _) => q
+  | (_, q, _, _, _) => q
 end.
 
-Definition get_paths (s: state) :=
+Definition get_dists (s: state) :=
   match s with
-  | (_, _, p) => p
+  | (_, _, d, _, _) => d
+  end.
+
+Definition get_time (s: state) :=
+  match s with
+  | (_, _, _, t, _) => t
+  end.
+
+Definition get_times (s: state) :=
+  match s with
+  |(_, _, _, _, t) => t
   end.
 
 Definition vertex_in (g: gr a b) (v: Graph.Node) : bool :=
   match (Graph.match_ v g) with | (None, _) => false | _ => true end.
 
-Definition in_graph (g : gr a b) (p: Graph.Path) : bool := 
-  match p with
-  | nil => false
-  | v :: xs => vertex_in g v  end. 
-
-Definition notIn_graph g := fun x => negb (in_graph g x). 
-
 Inductive bfs_step : state -> state -> Prop :=
-  | bfs_find: forall g l r (p: Graph.Path) (q' : list Graph.Path) c g' (v : Graph.Node) tl,
-    pop_list l (notIn_graph g) = p :: q' ->
-    p = v :: tl ->
-    Graph.match_ v g = (Some c, g') ->
-    bfs_step (g, l, r) (g', q' ++ (List.map (fun x => cons x p) (Graph.suc' c)), r ++ (p :: nil)).
+  | bfs_find: forall g d n t v j vs c g',
+      isEmpty g = false ->
+      match_ v g = (Some c, g') ->
+      bfs_step (g, (v, j) :: vs, d, n, t) (g', (vs ++ suci c (Num.op_zp__ j (Num.fromInteger 1))),
+        d ++ (v,j) :: nil, n + 1, (M.add v (n+1) t))
+  | bfs_skip: forall g d n t v j vs g',
+      isEmpty g = false ->
+      match_ v g = (None, g') ->
+      bfs_step (g, (v, j) :: vs, d, n, t) (g', vs, d, n, t).
 
-Definition start (g : gr a b) (v: Graph.Node) : state := (g, ((v :: nil) :: nil), nil).
+Definition start (g : gr a b) (v: Graph.Node) : state := (g, ((v, Num.fromInteger 0) :: nil), nil, 0, @M.empty nat).
 
 Inductive valid : state -> Node -> Prop :=
   | v_start : forall g v, vertex_in g v = true -> valid (start g v) v
@@ -139,209 +282,480 @@ Proof.
   intros. induction H0. assumption. apply IHmulti. eapply v_step. apply H. assumption.
 Qed.
 
-Definition natNodes (g : gr a b) := (BinInt.Z.abs_nat(Graph.noNodes g)).
+Definition done (s: state) := null (get_queue s) || isEmpty (get_graph s).
 
-Definition bfs_measure s := natNodes (get_graph s).
+(*Proof of correctness of bfs. Later, we prove equivalence between this inductive formulation and leveln,
+  allowing us to prove the correctness of this instead*)
+Section Correctness.
 
-Lemma step_decr_measure: forall s s',
-  bfs_step s s' ->
-  bfs_measure s' < bfs_measure s.
-Proof.
-  intros. inversion H; unfold bfs_measure; simpl.
-  eapply match_decr_size. symmetry. apply H2.
-Qed.
+(*Lots of stuff about paths here - TODO: move to separate file*)
+Section Path.
 
+(*Inductive and Fixpoint definitions for a path between two vertices. The Fixpoint instance proves that this is
+  decidable, and we prove their equivalence*)
+Inductive path : (gr a b) -> Node -> Node -> (list Node) -> Prop :=
+  | p_start: forall g u v, eIn g u v = true -> path g u v nil
+  | p_step: forall g u v w l, 
+     path g u w l ->
+     eIn g w v = true ->
+     path g u v (w :: l) .
 
-
-Definition next_state (s: state) : state :=
-  match s with
-  | (g, q, r) =>
-    let qnew := pop_list q (notIn_graph g) in
-    (*So it is same order as in haskell version*)
-    if (null qnew) then s else if (Graph.isEmpty g) then s else
-    match qnew with
-    (*impossible*)
-    | nil => s
-    | ((v :: tl) as p) :: q' => 
-      match (Graph.match_ v g) with
-       (*impossible*)
-       | (None, _) => s
-       | (Some c, g') => (g', q' ++ (List.map (fun x => cons x p) (Graph.suc' c)), r ++ (p :: nil))
-      end
-    (*impossible*)
-    | (nil :: q') => s
-    end
+Fixpoint path_list (g: gr a b) (u v: Node) (l: list Node) : bool :=
+  match l with
+  | nil => eIn g u v
+  | x :: tl => eIn g x v && path_list g u x tl
   end.
 
-Definition done (s: state) : bool :=
-  null (pop_list (get_queue s) (notIn_graph (get_graph s))) || (Graph.isEmpty (get_graph s)).
-
-(*Every path we create has at least 1 element (v)*)
-Lemma path_nonempty: forall s v,
-  valid s v ->
-  ~ In nil (get_paths s).
+Lemma path_list_equiv: forall g u v l,
+  path g u v l <-> path_list g u v l = true.
 Proof.
-  intros. intro. induction H.
-  - simpl in H0. destruct H0.
-  - inversion H1; subst.
-    + apply in_app_or in H0. destruct H0. apply IHvalid; simpl; assumption. simpl in H0. 
-      destruct H0. inversion H0. inversion H0.
+  intros. split; intros.
+  - induction H.
+    + simpl. assumption.
+    + simpl. rewrite andb_true_iff. split; assumption.
+  - generalize dependent v. induction l; intros; simpl.
+    + apply p_start. simpl in H. assumption.
+    + simpl in *. rewrite andb_true_iff in H. destruct H. apply p_step. apply IHl. assumption.
+      assumption.
 Qed.
 
-Lemma queue_path_nonempty: forall s v,
-  valid s v ->
-  ~ In nil (get_queue s).
+(*Some useful results about [path]*)
+Lemma path_app: forall g u v a l1 l2,
+  path_list g u v (l1 ++ a :: l2) = true <->
+  path_list g a v l1 = true /\ path_list g u a l2 = true.
 Proof.
-  intros. intro. induction H.
-  - simpl in H0. destruct H0. inversion H0. destruct H0.
-  - inversion H1; subst.
-    apply in_app_or in H0. destruct H0. simpl in IHvalid.
-     pose proof (pop_list_split l (notIn_graph g)). destruct H3 as [l']. destruct H3.
-    rewrite H2 in H3. apply IHvalid. rewrite <- H3. apply in_or_app. right.
-    simpl. right. assumption. 
-    assert (forall l, ~In nil (map (fun x : Node => x :: v0 :: tl) l)). { intros.
-    induction l0. simpl. auto. simpl. intro. destruct H3. inversion H3.
-    contradiction. } eapply H3. apply H0.
+  intros. split; intros. generalize dependent v. generalize dependent l2. induction l1; intros.
+  - simpl in H. simpl. rewrite andb_true_iff in H. apply H.
+  - simpl in *. simplify'; apply IHl1 in H1; destruct H1; assumption.
+  - destruct_all. generalize dependent v. generalize dependent a0. revert l2. induction l1; intros; simpl in *;
+    simplify'.
 Qed.
 
-
-Lemma next_step: forall s v, valid s v -> done s = false -> bfs_step s (next_state s).
+Lemma path_remove_cycle: forall g u v w l1 l2 l3,
+  path_list g u v (l1 ++ w :: l2 ++ w :: l3) = true ->
+  path_list g u v (l1 ++ w :: l3) = true.
 Proof.
-  intros. destruct s. destruct p as [g q]. simpl. unfold done in H0; simpl in H0.
-  rewrite Bool.orb_false_iff in H0. destruct H0. rewrite H0. rewrite H1.
-  destruct (pop_list q (notIn_graph g)) eqn : Q. inversion H0. 
-  simpl in H0. 
-  (*prove p = nil case impossible*)
-  destruct p eqn : P. pose proof (pop_list_split q (notIn_graph g)). destruct H2 as [l'].
-  destruct H2. rewrite Q in H2.  pose proof (queue_path_nonempty (g, q, r) v). 
-  apply H4 in H. simpl in H. rewrite <- H2 in H. exfalso. apply H. apply in_or_app. right.
-  simpl. left. reflexivity. destruct (match_ n g) eqn : M. assert (Q' := Q).
-  apply pop_split_fst in Q. unfold notIn_graph in Q. simpl in Q. unfold vertex_in in Q. rewrite M in Q.
-  destruct m. eapply bfs_find. apply Q'. reflexivity. apply M. inversion Q.
+  intros. apply path_app in H. destruct_all. apply path_app in H0. destruct_all.
+  apply path_app. simplify'.
+Qed.
+
+(*If there is a path, then there is a path with no duplicates*)
+Lemma path_no_dups: forall g u v l,
+  path_list g u v l = true ->
+  exists l1, path_list g u v l1 = true /\ NoDup l1 /\ ~In u l1 /\  ~In v l1 /\ 
+  (forall x, In x l1 -> In x l). 
+  Proof.
+    intros. induction l using (well_founded_induction
+                       (wf_inverse_image _ nat _ (@length _)
+                          PeanoNat.Nat.lt_wf_0)).
+    destruct (NoDup_dec (N.eq_dec) l).
+    - destruct (In_dec N.eq_dec u l).
+      + eapply in_split_app_fst in i. destruct_all. clear H2. subst.
+        apply path_app in H. destruct H. specialize (H0 x). destruct H0 as [l]. 
+        rewrite app_length. simpl. assert (forall n m, n < n + S(m)) by (intros; omega). apply H0.
+        apply H. exists l. simplify'. apply N.eq_dec.
+      + destruct (In_dec N.eq_dec v l).
+        * eapply in_split_app_fst in i. destruct_all; subst. clear H2. apply path_app in H.
+          destruct H. specialize (H0 x0). destruct H0 as [l]. rewrite app_length. simpl.
+          assert (forall n m, n < m + S(n)) by (intros; omega). apply H0. apply H1. exists l.
+          simplify'. apply N.eq_dec.
+        * exists l. simplify'.
+    - rewrite no_no_dup in n. destruct_all. subst. 
+      apply path_remove_cycle in H. specialize (H0 (x0 ++ x :: x2)). destruct H0 as [l].
+      repeat(rewrite app_length; simpl). omega. apply H. exists l. simplify'. apply H5 in H4.
+      apply in_app_or in H4. destruct H4. apply in_or_app. left. apply H4. simpl in H4.
+      destruct H4. subst. solve_in. solve_in. apply N.eq_dec.
+Qed.
+
+Lemma path_implies_in_graph: forall g u v l,
+  path_list g u v l = true ->
+  vIn g u = true /\ vIn g v = true /\ (forall x, In x l -> vIn g x = true).
+Proof.
+  intros. generalize dependent v. induction l; intros; simpl in H.
+  - apply edges_valid in H. simplify'.
+  - rewrite andb_true_iff in H. destruct H. apply IHl in H0. apply edges_valid in H. crush.
 Qed. 
 
-Lemma not_true: forall b,
-  b <> true -> b = false.
+
+(*We want a function to get the distance between two nodes. This is a horribly inefficient function to help do this*)
+(*A terrible function to find if a path of length <= n between two vertices exists*)
+Fixpoint path_of_length (g: gr a b) (u v : Node) (n: nat) {struct n} : bool :=
+  match n with
+  | 0 => eIn g u v
+  | S(m) => if eIn g u v then true else
+  fold_right (fun x t => if path_of_length g u x m && eIn g x v then true else t) false 
+  (nodeList g)
+  end.
+
+Lemma path_of_length_implies_path: forall g u v n,
+  path_of_length g u v n = true -> exists l, path_list g u v l = true /\ length l <= n.
 Proof.
-  intros. destruct b0; [contradiction | reflexivity].
+  intros. generalize dependent v. induction n; intros.
+  - simpl in H. exists nil. split. simpl. assumption. simpl. omega.
+  - simpl in H. destruct (eIn g u v) eqn : ?.
+    exists nil. split. simpl. assumption. simpl. omega.
+    assert (forall l, fold_right
+      (fun (x : Node) (t : bool) => if path_of_length g u x n && eIn g x v then true else t) false
+      l = true-> exists x, In x l /\ path_of_length g u x n = true /\ eIn g x v = true). {
+      intros. induction l; simpl in *.
+      * inversion H0.
+      * destruct (path_of_length g u a0 n && eIn g a0 v) eqn : ?.
+        -- exists a0. split. left. reflexivity. rewrite andb_true_iff in Heqb1. apply Heqb1.
+        -- apply IHl in H0. destruct H0. exists x. destruct H0. split. right. assumption.
+           apply H1. } 
+      apply H0 in H. clear H0. destruct H. destruct H. destruct H0. apply IHn in H0.
+      destruct H0. destruct H0. exists (x :: x0). split. simpl. rewrite andb_true_iff. crush. simpl. omega.
 Qed.
 
-(*The big one - a tail recursive version of BFS we want to prove equivalent to both the inductive version as well
-  as the Haskell one - Equations gives nice rewrite rules and elimination rules to prove things with this
-  definition more easily*)
-Equations bfs_tail (s: state) v (H: valid s v) : state by wf (bfs_measure s) lt :=
-  bfs_tail s v H := if bool_dec (done s) true then s else (bfs_tail (next_state s) v _).
-Next Obligation.
-eapply v_step. apply H. eapply next_step. apply H. apply not_true; assumption. 
-Defined.
-Next Obligation.
-apply step_decr_measure. eapply next_step. apply H. apply not_true; assumption.
-Defined.
-
-(*Prove valid and done*)
-Lemma bfs_tail_done: forall s v (H: valid s v),
-  done (bfs_tail s v H) = true.
+Lemma path_of_size_implies_function: forall g u v l n,
+  length l <= n ->
+  path_list g u v l = true -> path_of_length g u v n = true.
 Proof.
-  intros. apply bfs_tail_elim. intros. destruct (bool_dec (done s0) true) eqn : ?.
-  apply e. apply H1.
+  intros. generalize dependent v. revert u. generalize dependent n. induction l; simpl in *; intros.
+  - destruct n. simpl. apply H0. simpl. rewrite H0. reflexivity.
+  - simplify. destruct n. omega. assert (length l <= n) by omega. clear H.
+    simpl. destruct (eIn g u v) eqn : ?. reflexivity.
+      assert (forall a l', In a l' ->
+      path_of_length g u a n = true ->
+      eIn g a v = true ->
+      fold_right
+  (fun (x : Node) (t : bool) => if path_of_length g u x n && eIn g x v then true else t)
+  false l' = true). { intros. induction l'; simpl in *.
+  - destruct H.
+  - destruct H. subst. rewrite H3. rewrite H2. simpl. reflexivity. apply IHl' in H. 
+    destruct (path_of_length g u a2 n && eIn g a2 v). reflexivity. apply H. }
+    apply (H a0). assert (vIn g a0 = true). { rewrite andb_true_iff in H0.
+    destruct H0. apply edges_valid in H0. apply H0. } unfold vIn in H2.
+    unfold mem in H2. destruct (in_dec N.eq_dec a0 (nodeList g)) eqn : ?. assumption.
+    rewrite Heqs in H2. inversion H2. apply IHl. apply H1. simplify'. simplify'.
 Qed.
 
-Lemma bfs_tail_multi: forall s v (H: valid s v),
-  bfs_multi s (bfs_tail s v H).
+(*If there is a path, then there is a path at most as large as the number of vertices in the graph (because
+  there is a path with no duplicates and every vertex is in the graph*)
+Lemma path_shorter_than_graph_size: forall g u v l,
+  path_list g u v l = true ->
+  exists l', path_list g u v l' = true /\ length l' <= length(nodeList g).
 Proof.
-  intros. apply bfs_tail_elim. intros. destruct (bool_dec (done s0) true) eqn : ?.
-  - apply multi_refl.
-  - eapply multi_step. eapply next_step. apply H0. apply not_true; assumption. apply H1.
+  intros. apply path_no_dups in H. destruct_all. 
+  assert (forall a, In a x -> In a (nodeList g)). intros.
+  apply path_implies_in_graph in H. destruct_all. apply H6 in H4. unfold vIn in H4.
+  unfold mem in H4. destruct (in_dec N.eq_dec a0 (nodeList g)) eqn : ?. assumption.
+  rewrite Heqs in H4. inversion H4. 
+  exists x. split. apply H. eapply NoDup_incl_length. apply H0. unfold incl. apply H4.
 Qed.
 
-(*Well formed lexicographic measure - maybe put in own section*)
+(*By the above lemma, we can simply define distance by repeatedly checking if there is a list with 
+  the given distance*)
+Definition distance (g: gr a b) (u v : Node) : option nat :=
+  fold_right (fun x acc => if path_of_length g u v x then Some x else acc) None (seq 0 (natNodes g + 1)).
 
-
-Definition natNodes_lt x y := natNodes x < natNodes y.
-Definition natNodes_eq x y := natNodes x = natNodes y.
-Definition list_length_lt {a} (x y : list a) := length x < length y.
-Definition queue_length_lt  {a} (x y : Queue a) := list_length_lt (toList _ x) (toList _ y).
-
-Definition bf_measure_list := 
-  transp (lex (transp natNodes_lt) natNodes_eq (transp  (@list_length_lt Path))).
-
-Definition bf_measure_queue :=
-  transp (lex (transp natNodes_lt) natNodes_eq (transp (@queue_length_lt Path))).
-
-Definition f_nat_lt {a} (f: a -> nat) x y := f x < f y.
-
-Lemma f_nat_lt_acc: forall {a} (f: a -> nat) x n, f x <= n -> Acc (f_nat_lt f) x.
+Lemma distance_none: forall g u v,
+  distance g u v = None <-> (forall l, path_list g u v l = false).
 Proof.
-  intros. generalize dependent x. induction n; auto.
-  - intros. apply Acc_intro. intros. unfold f_nat_lt in *. omega.
-  - unfold f_nat_lt in *. intros. apply Acc_intro. intros. apply IHn. omega.
+  intros.  assert (A: forall l, fold_right (fun (x : nat) (acc : option nat) => 
+    if path_of_length g u v x then Some x else acc) None l = None <->
+    (forall x, In x l -> path_of_length g u v x = false)). { intros. split; intros; induction l; simpl in *.
+    destruct H0. destruct H0. subst. destruct (path_of_length g u v x) eqn : ?. inversion H.
+    reflexivity. apply IHl. destruct (path_of_length g u v a0) eqn : ?. inversion H.
+    apply H. assumption. reflexivity. destruct (path_of_length g u v a0) eqn : ?.
+    specialize (H a0). rewrite H in Heqb0. inversion Heqb0. left. reflexivity.
+    apply IHl. intros. apply H. right. assumption. } 
+     split; intros.
+  - unfold distance in H. 
+    assert (forall x, In x (seq 0 (natNodes g + 1)) -> path_of_length g u v x = false). { intros.
+    eapply A. apply H. assumption. } clear H. clear A.
+    destruct (path_list g u v l) eqn : P.
+    + apply path_shorter_than_graph_size in P. destruct P. destruct H.
+      assert (path_of_length g u v (length x) = true). eapply path_of_size_implies_function.
+      reflexivity. assumption. 
+      assert (In (length x) (seq 0 (natNodes g + 1))). apply in_seq. split. omega. simpl.
+      assert (length (nodeList g) = natNodes g). unfold natNodes. rewrite noNodes_def. 
+      unfold nodeList. unfold ulabNodes. apply map_length. omega. 
+      apply H0 in H3. rewrite H3 in H2. inversion H2.
+    + reflexivity.
+  - unfold distance. apply A. intros. destruct (path_of_length g u v x) eqn : ?.
+    + apply path_of_length_implies_path in Heqb0. destruct Heqb0. destruct H1. rewrite H in H1.
+      inversion H1.
+    + reflexivity.
 Qed.
 
-Lemma f_nat_lt_wf: forall {a} (f: a -> nat), well_founded (f_nat_lt f).
+Lemma seq_pred: forall start len h t n l,
+  seq start len = (h :: t) ++ S n :: l ->
+  In n (h :: t).
 Proof.
-  red. intro. intro. intro. eapply f_nat_lt_acc. eauto.
+  intros. generalize dependent h. revert t. revert start0. induction len; intros.
+  - simpl. simpl in H. inversion H.
+  - simpl in H. inversion H. subst. destruct t.
+    simpl in H2. simpl. destruct len. simpl in H2. inversion H2. simpl in H2. inversion H2. subst. left. reflexivity.
+    apply IHlen in H2. solve_in.
 Qed.
 
-
-Lemma wf_bf_measure_list : WF (transp bf_measure_list).
+Lemma seq_split: forall start len l1 x l2,
+  seq start len = l1 ++ x :: l2 ->
+  (forall y, In y l1 -> y < x) /\ (forall y, In y l2 -> y > x).
 Proof.
-  eapply WF_lex.
-  - apply wf_transp_WF. unfold transp. 
-    pose proof (f_nat_lt_wf (natNodes)). unfold f_nat_lt in H. unfold natNodes_lt. apply H.
-  - apply wf_transp_WF. unfold transp.
-    pose proof (f_nat_lt_wf (@length Path)). unfold f_nat_lt in H. unfold natNodes_lt. apply H.
-  - unfold Transitive. intros. unfold natNodes_eq in *. omega.
-  - unfold inclusion. unfold RelUtil.compose. intros.
-    unfold transp in *. unfold natNodes_lt in *. unfold natNodes_eq in *. destruct H. omega.
+  intros. generalize dependent start0. revert l1. revert x. revert l2. induction len; intros; simpl in H.
+  - assert (l1 = nil). destruct l1; inversion H. subst.
+    simpl in H. inversion H.
+  - destruct l1. simpl in H. inversion H. destruct l2.
+     split; intros. destruct H0. rewrite H2 in H0. destruct H0.
+     specialize (IHlen l2 n nil (S(start0))). subst. simpl in IHlen. apply IHlen in H2.
+     split; intros. destruct H0. rewrite in_seq in H0. omega.
+     inversion H; subst. specialize (IHlen l2 x l1 (S(n)) H2). split; intros. simpl in H0.
+     destruct H0. subst. assert (In x (seq (S(y)) len)). rewrite H2. solve_in. rewrite in_seq in H0.
+      omega. destruct IHlen. apply H1. assumption. apply IHlen. apply H0.
 Qed.
 
-Lemma well_founded_bf_measure_list: well_founded (bf_measure_list).
+(*This actually computes the shortest path*)
+Lemma distance_some: forall g u v n,
+  distance g u v = Some n <->
+  (exists l, path g u v l /\ length l = n) /\ (forall l, length l < n -> path_list g u v l = false).
 Proof.
-  apply WF_transp_wf. apply wf_bf_measure_list.
-Qed.
+  intros. unfold distance.
+  assert (forall l, 
+  fold_right (fun (x : nat) (acc : option nat) => if path_of_length g u v x then Some x else acc) None
+  l = Some n <-> (exists l1 l2, l = l1 ++ n :: l2 /\ (forall y, In y l1 -> path_of_length g u v y = false) /\
+  path_of_length g u v n = true)). { intros. induction l; split; intros; simpl in *.
+  - inversion H.
+  - destruct_all. destruct x; inversion H.
+  - destruct (path_of_length g u v a0) eqn : ?.
+    + inversion H; subst. exists nil. exists l. split. simpl. reflexivity. split; intros.
+      destruct H0. assumption.
+    + apply IHl in H. destruct H. exists (a0 :: x). destruct_all.
+      exists x0. split. rewrite H. simpl. reflexivity.
+      split; intros. simpl in H2. destruct H2. subst. assumption. apply H0. assumption.
+      assumption.
+  - destruct_all. destruct (path_of_length g u v a0) eqn : ?. destruct x.
+    + inversion H; subst. reflexivity.
+    + simpl in H0. inversion H; subst. specialize (H0 n0). rewrite H0 in Heqb0. inversion Heqb0.
+      left. reflexivity.
+    + destruct x. inversion H; subst. rewrite Heqb0 in H1. inversion H1.
+      inversion H; subst. apply IHl. exists x. exists x0. simplify'. }
+  rewrite H. clear H. split; intros; destruct_all.
+  - apply path_of_length_implies_path in H1. split. setoid_rewrite path_list_equiv. 
+    destruct  H1. destruct H1. assert (length x1 = n \/ length x1 < n) by omega. destruct H3.
+    exists x1. split. assumption. assumption. 
+    destruct x. simpl in H. assert (natNodes g + 1 = S(natNodes g)) by omega. rewrite H4 in H.
+    simpl in H. inversion H; subst. omega. 
+    destruct n. omega. assert (length x1 <= n) by omega. 
+    apply (path_of_size_implies_function _ _ _ _ _ H4) in H1.
+    rewrite H0 in H1. inversion H1. apply seq_pred in H. apply H.
+    intros. assert (In (length l) (seq 0 (natNodes g + 1))). { rewrite in_seq.
+    assert (In n (seq 0 (natNodes g + 1))). rewrite H. solve_in. rewrite in_seq in H3.
+    omega. } rewrite H in H3. apply seq_split in H.
+    destruct H. apply in_app_or in H3. destruct H3. 
+    destruct (path_list g u v l) eqn : ?. eapply path_of_size_implies_function in Heqb0.
+    rewrite (H0 (length l)) in Heqb0. inversion Heqb0.
+    assumption. omega. reflexivity. simpl in H3. destruct H3. omega.
+    apply H4 in H3. omega.
+  - assert (n <= (natNodes g)). { assert (n <= natNodes g \/ n > natNodes g) by omega. destruct H2.
+    assumption. rewrite path_list_equiv in H. apply path_shorter_than_graph_size in H.
+    destruct H. destruct H. rewrite H0 in H. inversion H. unfold nodeList in H3.
+    unfold ulabNodes in H3. rewrite map_length in H3. rewrite <- noNodes_def in H3.
+    unfold natNodes in H2. omega. }
+    pose proof (in_split_app_fst _ (seq 0 (natNodes g + 1)) n Nat.eq_dec).
+    assert (In n (seq 0 (natNodes g + 1))). rewrite in_seq. omega.
+    apply H3 in H4. clear H3. destruct_all. exists x0. exists x1. split. assumption.
+    apply seq_split in H3. split; intros.
+    destruct H3. destruct (path_of_length g u v y) eqn : ?.
+    apply path_of_length_implies_path in Heqb0. destruct Heqb0.
+    destruct H7. rewrite H0 in H7. inversion H7. apply H3 in H5. omega. reflexivity.
+    eapply path_of_size_implies_function. assert (length x <= n) by omega. apply H5.
+    rewrite <- path_list_equiv. assumption.
+Qed. 
 
-Lemma wf_bf_measure_queue : WF (transp bf_measure_queue).
-Proof.
-  eapply WF_lex.
-  - apply wf_transp_WF. unfold transp. 
-    pose proof (f_nat_lt_wf (natNodes)). unfold f_nat_lt in H. unfold natNodes_lt. apply H.
-  - apply wf_transp_WF. unfold transp.
-    pose proof (f_nat_lt_wf (fun x => length (toList Path x))). unfold f_nat_lt in H. unfold queue_length_lt.
-    unfold list_length_lt. apply H.
-  - unfold Transitive. intros. unfold natNodes_eq in *. omega.
-  - unfold inclusion. unfold RelUtil.compose. intros.
-    unfold transp in *. unfold natNodes_lt in *. unfold natNodes_eq in *. destruct H. omega.
-Qed.
 
-Lemma well_founded_bf_measure_queue: well_founded (bf_measure_queue).
-Proof.
-  apply WF_transp_wf. apply wf_bf_measure_queue.
-Qed.
+(*Next step lemma 22.1 of CLRS*)
 
+End Path.
 
-Instance need_this_for_equations : WellFounded bf_measure_list.
+End Correctness.
+
+Section Equiv.
+
+Instance need_this_for_equations : WellFounded (bf_measure_list (Node * Num.Int)).
 Proof.
   unfold WellFounded. apply well_founded_bf_measure_list.
 Defined.
 
-
-Axiom match_None1: forall (g: gr a b) v g',
-  match_ v g = (None, g') -> Graph.Desc g' (noNodes g) (fun x => vIn g x) (fun x y => eIn g x y).
-
-Axiom match_None2: forall (g: gr a b) v,
-  (exists g', match_ v g = (None, g')) <-> ~vIn g v.
-
-(*should prove this from others ,also may have to change edge thing because of multiple edges*)
-Axiom match_None3: forall (g: gr a b) v g',
-  match_ v g = (None, g') -> noNodes g = noNodes g'.
-
 Lemma match_none_size: forall g v g',
   match_ v g = (None, g') -> natNodes g = natNodes g'.
 Proof.
-  intros. unfold natNodes. erewrite match_None3. reflexivity. apply H.
+  intros. pose proof (match_remain_none g). erewrite H0. reflexivity. apply H.
+Qed.  
+
+Equations bfs_tail (s: state) : state by wf (get_graph s, get_queue s) (bf_measure_list (Node * Num.Int)) :=
+  bfs_tail (g, nil, x, y, z) => (g, nil, x, y, z);
+  bfs_tail (g, (v, j) :: vs, d, n, t) => if (isEmpty g) then  (g, (v, j) :: vs, d, n, t) else
+      match (match_ v g) as y return ((match_ v g = y) -> _) with
+      | (Some c, g') => fun H: (match_ v g) = (Some c, g') => 
+        bfs_tail (g', (vs ++ suci c (Num.op_zp__ j (Num.fromInteger 1))), d ++ (v,j) :: nil, n + 1, M.add v (n+1) t)
+      | (None, g') => fun H: (match_ v g) = (None, g') => bfs_tail (g', vs, d, n, t)
+      end (eq_refl).
+Next Obligation.
+unfold bf_measure_list. unfold transp. apply lex1. unfold natNodes_lt. eapply match_decr_size. symmetry. apply H.
+Defined.
+Next Obligation.
+unfold bf_measure_list. unfold transp. apply lex2. unfold natNodes_eq. eapply match_none_size. apply H. unfold list_length_lt.
+simpl. omega.
+Defined.
+
+Definition expand_bfs_tail := 
+fun s : gr a b * list (Node * Num.Int) * list (Node * Num.Int) * nat * M.t nat =>
+let (p, t) := s in
+(let (p0, n) := p in
+ fun t0 : M.t nat =>
+ (let (p1, l) := p0 in
+  fun (n0 : nat) (t1 : M.t nat) =>
+  (let (g, l0) := p1 in
+   fun (l1 : list (Node * Num.Int)) (n1 : nat) (t2 : M.t nat) =>
+   match l0 with
+   | nil => fun (l2 : list (Node * Num.Int)) (n2 : nat) (t3 : M.t nat) => (g, nil, l2, n2, t3)
+   | p2 :: l2 =>
+       fun (l3 : list (Node * Num.Int)) (n2 : nat) (t3 : M.t nat) =>
+       (let (n3, i) := p2 in
+        fun (l4 l5 : list (Node * Num.Int)) (n4 : nat) (t4 : M.t nat) =>
+        if isEmpty g
+        then (g, (n3, i) :: l4, l5, n4, t4)
+        else
+         (let
+            (m, g') as y
+             return (match_ n3 g = y -> gr a b * list (Node * Num.Int) * list (Node * Num.Int) * nat * M.t nat) :=
+            match_ n3 g in
+          match
+            m as m0
+            return
+              (match_ n3 g = (m0, g') -> gr a b * list (Node * Num.Int) * list (Node * Num.Int) * nat * M.t nat)
+          with
+          | Some c =>
+              fun _ : match_ n3 g = (Some c, g') =>
+              bfs_tail
+                (g', l4 ++ suci c (Num.op_zp__ i (Num.fromInteger 1)), l5 ++ (n3, i) :: nil, 
+                n4 + 1, M.add n3 (n4 + 1) t4)
+          | None => fun _ : match_ n3 g = (None, g') => bfs_tail (g', l4, l5, n4, t4)
+          end) eq_refl) l2 l3 n2 t3
+   end l1 n1 t2) l n0 t1) n t0) t.
+
+Lemma unfold_bfs_tail: forall s,
+  bfs_tail s = expand_bfs_tail s.
+Proof.
+  intros. unfold expand_bfs_tail. apply bfs_tail_elim; intros; reflexivity.
+Qed.
+
+(*Want to prove this is valid, done and equivalent to other*)
+Lemma bfs_tail_multi: forall s,
+  bfs_multi s (bfs_tail s).
+Proof.
+  intros. destruct s as [r t]. destruct r as [r n]. destruct r as [r d].
+  generalize dependent d. revert n. revert t. 
+   induction (r) using (well_founded_induction (well_founded_bf_measure_list (Node * Num.Int))).
+  intros.
+  destruct r as [g q]. rewrite unfold_bfs_tail. simpl. destruct q eqn : Q.
+  - apply multi_refl.
+  - destruct p as [v j]. destruct (isEmpty g) eqn : E.
+    + apply multi_refl.
+    + destruct (match_ v g) eqn : M. destruct m eqn : M'.
+      *  eapply multi_step. apply bfs_find. assumption. apply M. apply H. unfold bf_measure_list.
+         unfold transp. apply lex1. unfold natNodes_lt. eapply match_decr_size. symmetry. apply M.
+      * eapply multi_step. apply bfs_skip. assumption. apply M. apply H. unfold bf_measure_list.
+        unfold transp. apply lex2. unfold natNodes_eq. eapply match_none_size; eassumption.
+        unfold list_length_lt. simpl. omega.
+Qed.  
+
+Lemma bfs_tail_done: forall s,
+  done (bfs_tail s) = true.
+Proof.
+  intros. unfold done. destruct s as [r t]. destruct r as [r n]. destruct r as [r d].
+  generalize dependent d. revert n. revert t. 
+   induction (r) using (well_founded_induction (well_founded_bf_measure_list (Node * Num.Int))).
+  intros.
+  destruct r as [g q]. rewrite unfold_bfs_tail. simpl. destruct q eqn : Q.
+  - simpl. reflexivity.
+  - destruct p. simpl. destruct (isEmpty g) eqn : G. simpl. assumption.
+    destruct (match_ n0 g) eqn : M. destruct m; simpl.
+    apply H. unfold bf_measure_list. unfold transp. apply lex1. unfold natNodes_lt. eapply match_decr_size;
+    symmetry; eassumption. apply H. unfold bf_measure_list. unfold transp. apply lex2.
+    unfold natNodes_eq. eapply match_none_size. eassumption. unfold list_length_lt. simpl. omega.
 Qed. 
 
-Equations bf_list (x : (gr a b) * (list Path)) : RootPath.RTree by wf x bf_measure_list :=
+(*Equivalence of 2 versions - TODO: prove leveln and leveln' equivalent (proof is basically what I did before*)
+Equations leveln' (x: (gr a b) * (list (Node * Num.Int))) : list (Node * Num.Int) by wf x (bf_measure_list (Node * Num.Int)) :=
+  leveln' (g, nil) := nil;
+  leveln' (g, (v,j) :: vs) := if (isEmpty g) then nil else
+                                match (match_ v g) as y return ((match_ v g = y) -> _ ) with
+                                | (Some c, g') => fun H : (match_ v g) = (Some c, g') => (v,j) :: leveln' (g', (vs ++ suci c (Num.op_zp__ j (Num.fromInteger 1))))
+                                | (None, g') => fun H: (match_ v g) = (None, g') => leveln' (g', vs)
+                                 end (eq_refl).
+Next Obligation.
+unfold bf_measure_list. unfold transp. apply lex1. unfold natNodes_lt. eapply match_decr_size. symmetry. apply H.
+Defined.
+Next Obligation.
+unfold bf_measure_list. unfold transp. apply lex2. unfold natNodes_eq. eapply match_none_size. apply H. unfold list_length_lt.
+simpl. omega.
+Defined.
+
+Definition expand_leveln' := 
+fun x : gr a b * list (Node * Num.Int) =>
+let (g, l) := x in
+match l with
+| nil => nil
+| p :: l0 =>
+    (let (n, i) := p in
+     fun l1 : list (Node * Num.Int) =>
+     if isEmpty g
+     then nil
+     else
+      (let (m, g') as y return (match_ n g = y -> list (Node * Num.Int)) := match_ n g in
+       match m as m0 return (match_ n g = (m0, g') -> list (Node * Num.Int)) with
+       | Some c =>
+           fun _ : match_ n g = (Some c, g') =>
+           (n, i) :: leveln' (g', l1 ++ suci c (Num.op_zp__ i (Num.fromInteger 1)))
+       | None => fun _ : match_ n g = (None, g') => leveln' (g', l1)
+       end) eq_refl) l0
+end.
+
+Lemma unfold_leveln': forall x,
+  leveln' x = expand_leveln' x.
+Proof.
+  intros. unfold expand_leveln'. apply leveln'_elim. reflexivity. reflexivity.
+Qed.
+
+Lemma leveln_tail_equiv: forall x l n t,
+  get_dists (bfs_tail (x, l, n, t)) = l ++ leveln' x.
+Proof.
+  intros x. 
+  induction (x) using (well_founded_induction (well_founded_bf_measure_list (Node * Num.Int))).
+  intros. rewrite unfold_leveln'. rewrite unfold_bfs_tail. simpl. unfold expand_leveln'.
+  destruct x as [g q]. simpl. destruct q eqn : Q.
+  - simpl. rewrite app_nil_r. reflexivity.
+  - destruct p as [v j]. destruct (isEmpty g) eqn : G. 
+    + simpl. rewrite app_nil_r. reflexivity.
+    + destruct (match_ v g) eqn : M. destruct m.
+      * remember (g0, l0 ++ suci c (j + 1)%Z) as x. rewrite H. rewrite <- app_assoc. simpl.
+        reflexivity. unfold bf_measure_list.  unfold transp. simpl. destruct x. apply lex1.
+        unfold natNodes_lt. eapply match_decr_size. symmetry. inversion Heqx; subst. apply M.
+      * rewrite H. reflexivity. unfold bf_measure_list. unfold transp. apply lex2.
+        unfold natNodes_eq. eapply match_none_size. apply M. unfold list_length_lt. simpl. omega.
+Qed. 
+
+(*Need to wait until I prove equivalence of leveln and leveln', but easy from there*)
+Theorem level_tail_equiv: forall v g,
+  get_dists (bfs_tail (start g v)) = level v g.
+Proof.
+Abort.
+
+End Equiv.
+
+(*BFS with paths - come back to this*)
+
+Section WithPath.
+
+Instance also_need_this_for_equations : WellFounded (bf_measure_list (Path)).
+Proof.
+  unfold WellFounded. apply well_founded_bf_measure_list.
+Defined.
+
+Equations bf_list (x : (gr a b) * (list Path)) : RootPath.RTree by wf x (bf_measure_list Path) :=
   bf_list (g, nil) := nil;
   bf_list (g, (nil :: q')) := if (isEmpty g) then nil else GHC.Err.patternFailure;
   bf_list (g, ((v :: t) :: q')) := let p:= v :: t in  if (isEmpty g) then nil else
@@ -359,12 +773,6 @@ Next Obligation.
 unfold bf_measure_list. unfold transp. apply lex2. unfold natNodes_eq. eapply match_none_size. apply H.
 unfold list_length_lt. simpl. omega.
 Defined.
-
-(*Defn*)
-Print bf_list_unfold.
-Check bf_list_unfold_eq.
-(*could be useful*)
-Check bf_list_elim.
 
 
 
@@ -456,12 +864,12 @@ Lemma bf_list_equiv: forall (x: (gr a b) * (Queue Path)),
   bf_strict'  (fst x) (snd x) = bf_list ((fst x), (toList _ (snd x))).
 Proof.
   intros. unfold bf_strict'. rewrite <- bf_list_unfold'_equiv. simpl.
-  induction (x) as [y IH] using (well_founded_induction well_founded_bf_measure_queue). 
+  induction (x) as [y IH] using (well_founded_induction (well_founded_bf_measure_queue (Path))). 
   destruct y as [g q]. simpl. unfold deferredFix2 in *. unfold curry in *.
-  rewrite (deferredFix_eq_on _ (fun x => True) ( bf_measure_queue )).
+  rewrite (deferredFix_eq_on _ (fun x => True) ( (bf_measure_queue (Path)) )).
   - simpl. destruct (toList _ q) eqn : Q.  
     + simpl. assert (queueEmpty q = true). rewrite toList_queueEmpty. assumption. rewrite H.
-      reflexivity.
+      simpl. reflexivity.
     + simpl. assert (queueEmpty q = false). destruct (queueEmpty q) eqn : ?. rewrite toList_queueEmpty in Heqb0.
       rewrite Heqb0 in Q. inversion Q. reflexivity. rewrite H. simpl.
       destruct (isEmpty g) eqn : GE. destruct p; reflexivity.
@@ -498,6 +906,28 @@ Lemma bf_list_equiv': forall (g: gr a b) (q: Queue Path),
 Proof.
   intros. pose proof (bf_list_equiv (g, q)). simpl in H. assumption.
 Qed. 
+
+Lemma contrapositive: forall (P Q : Prop), (P -> Q) -> (~Q -> ~P).
+Proof.
+  tauto.
+Qed. 
+(*probably dont need this*)
+Lemma bf_list_unroll: forall (g: gr a b) (l: list Path) n p t,
+  l = (n :: p) :: t ->
+  vIn g n = false ->
+  bf_list (g, l) = bf_list (g, t).
+Proof.
+  intros. rewrite <- bf_list_unfold'_equiv at 1. simpl.
+  rewrite H. destruct (isEmpty g) eqn : G.
+  rewrite <- bf_list_unfold'_equiv. simpl. destruct t. reflexivity.
+  destruct l0. rewrite G. reflexivity. rewrite G. reflexivity.
+  destruct (match_ n g) eqn : M. destruct m.
+  - pose proof (match_in g n). destruct H1. apply contrapositive in H1.
+    exfalso. apply H1. exists c. exists g0. assumption. intro. rewrite H3 in H0. inversion H0.
+  - pose proof (match_remain_none g n g0 M). subst. reflexivity.
+Qed.
+
+End WithPath.
 
 (*Equivalence*)
 
